

$$(f + g)' = f' + g'$$
$$(fg)' = f \cdot g' + f' \cdot g$$
$$(f \circ g)' = (f' \circ g) \cdot g'$$
$$\left(\frac{f}{g}\right) = \frac{g \cdot f' - f \cdot g'}{g^{2}}$$

## Ableitung von Potenzreihen

$$\begin{align*}
&P(x) = \sum\limits^{\infty}_{n=0} a_{n} x^{n}\\
&P'(x) = \sum\limits^{\infty}_{n=1} n \cdot a_{n}\cdot x^{n-1}\\
	&= \sum\limits^{\infty}_{n=0} (n+1) a_{n+1} x^{n}
\end{align*}$$

## Sinus und Cosinus Abbleitungen

$$\begin{align*}
\cos(x) &= \sum\limits^{\infty}_{n=0} \frac{(-1)^{n}}{(2n)!} x ^{2n}\\
\cos'(x) &= \sum\limits^{\infty}_{n=1}  \frac{(-1)^{n}}{(2n-1)}!x^{2n-1}\\
-\sum\limits^{\infty}_{n=0} \frac{(-1)^{n}}{(2n-1)!} x^{2n+1} &= -\sin(x)=
\end{align*}$$

## Logarithmus

$$\begin{align*}
\ln(x) &= \sum\limits^{\infty}_{n=1} \frac{(-1)^{n-1}}{n} (x-1)^n\\
\ln'(x) &= \sum\limits^{\infty}_{n=1}(-1)^{n-1} (x-1)^{n-1} &= \sum\limits^{\infty}_{n=0} (1-x)^{n}&= \frac{1}{1-(1-x)} &= \frac{1}{x}
\end{align*}$$



