

$$\begin{align*}
&\left(\begin{array}x_{1} \\ \vdots \\ x_n\end{array}\right) \in \mathbb R^n\\
&\implies \left(\begin{array}
x_{y}+ y_{1}\\ \vdots \\ x_{n}+ y_n
\end{array}\right)\\
&\implies \left(\begin{array}
\lambda x_{1}\\\vdots \\ \lambda x_{n}
\end{array}\right)
\end{align*}$$

$$\sum\limits_{j=1}^{n} a_{i,j}\; x_{j}= 0 \qquad \forall i=1, ... r $$


$$\begin{align*}
\forall i=1, ..., r \sum\limits_{i=1}^{n} a_{i,j} x_{j}= 0 \qquad\sum\limits_{j=1}^{n} a_{i,j} \; y_{j}= 0\\
\sum\limits^{n}_{j=1} a_{i,j}\; (x_{j}+ y_{j}) = \underbrace{\sum\limits^{n}_{j=1} a_{i,j} y_{j}}_{0} + \underbrace{\sum\limits^{n}_{j=1}a_{i,j}}_{0}\; y_{j} &= 0 \quad\forall i
\end{align*}
$$


