


|                                                             | a                                                                                                                                  | b                                                                                                                                                 | c                                                                                                                                                                 |
| ----------------------------------------------------------- | ---------------------------------------------------------------------------------------------------------------------------------- | ------------------------------------------------------------------------------------------------------------------------------------------------- | ----------------------------------------------------------------------------------------------------------------------------------------------------------------- |
| $p_\top$                                                    | $\top$                                                                                                                             | $\top$                                                                                                                                            | $\top$                                                                                                                                                            |
| $p_\bot$                                                    | $\bot$                                                                                                                             | $\bot$                                                                                                                                            | $\bot$                                                                                                                                                            |
| $p_a$                                                       | $p_\top$                                                                                                                           | $\bot$                                                                                                                                            | $\bot$                                                                                                                                                            |
| $p_{\neg a}$                                                | $p_\bot$                                                                                                                           | $\top$                                                                                                                                            | $\top$                                                                                                                                                            |
| $p_b$                                                       | $\bot$                                                                                                                             | $p_\top$                                                                                                                                          | $\bot$                                                                                                                                                            |
| $p_{\neg b}$                                                | $\top$                                                                                                                             | $p_\bot$                                                                                                                                          | $\top$                                                                                                                                                            |
| $p_c$                                                       | $\bot$                                                                                                                             | $\bot$                                                                                                                                            | $p_\top$                                                                                                                                                          |
| $p_{\neg c}$                                                | $\top$                                                                                                                             | $\top$                                                                                                                                            | $p_\bot$                                                                                                                                                          |
| $p_{b\lor c}$                                               | $\bot$                                                                                                                             | $p_\top \lor \bot$                                                                                                                                | $\bot \lor p_\top$                                                                                                                                                |
| $p_{\neg(b\lor c)}$                                         | $\top$                                                                                                                             | $p_\bot$                                                                                                                                          | $p_\bot$                                                                                                                                                          |
| $p_{\top U (b \lor c)}$                                     | $\bot \lor (\top \land p_{\top U (b \lor c)})$                                                                                     | $(p_\top  \lor \bot)\lor (\top \land p_{\top U (b \lor c)})$                                                                                      | $(\bot \lor p_\top \lor (\top \land p_{\top U (b \lor c)})$                                                                                                       |
| $p_{\neg(\top U (b \lor c))}$                               | $\top \land (\bot \lor p_{\neg(\top U (b \lor c))})$                                                                               | $(p_\bot\land \top) \land(\bot \lor p_{\neg (\top U (b\lor c))})$                                                                                 | $(\top \land p_\bot) \land (\bot \lor p_{\neg (\top U (b\lor c))})$                                                                                               |
| $p_{a \land \neg (\top U (b\lor c))}$                       | $p_\top \land (\top \land (\bot \lor p_{\neg(\top U (b \lor c))}))$                                                                | $\bot \land ((p_\bot\land \top) \land(\bot \lor p_{\neg (\top U (b\lor c))}))$                                                                    | $\bot \land ((\top \land p_\bot) \land (\bot \lor p_{\neg (\top U (b\lor c))}))$                                                                                  |
| $p_{\neg(a \land \neg (\top U (b\lor c)))}$                 | $p_\bot \lor (\bot \lor (\top \land p_{\top U (b \lor c)}))$                                                                       | $\top \lor ((p_\top  \lor \bot)\lor (\top \land p_{\top U (b \lor c)}))$                                                                          | $\top \lor (\bot \lor p_\top \lor (\top \land p_{\top U (b \lor c)})$                                                                                             |
| $p_{\top U (a \land \neg (\top U (b\lor c)))}/p_{\neg\phi}$ | $p_\top \land (\top \land (\bot \lor p_{\neg(\top U (b \lor c))})) \lor (\top \land p_{\top U (a \land \neg (\top U (b\lor c)))})$ | $(\bot \land ((p_\bot\land \top) \land(\bot \lor p_{\neg (\top U (b\lor c))}))) \lor (\top \land p_{\top U (a \land \neg (\top U (b\lor c)))})$   | $(\bot \land ((p_\bot\land \top) \land(\bot \lor p_{\neg (\top U (b\lor c))}))) \lor (\top \lor (\bot \lor p_\top \lor (\top \land p_{\top U (b \lor c)})))$      |
| $p_{\neg(\top U (a \land \neg (\top U (b\lor c))))}/p_\phi$ | $p_\bot \lor (\top \land (\top \land p_{\top U (b \lor c)})) \land (\bot \lor p_{\neg (\top U (a \land \neg \top U (b \lor c)))})$ | $(\top \lor (( p_\top \lor \bot) \land (\top \land p_{\top U (b \lor c)}))) \land (\bot \lor p_{\neg (\top U (a \land \neg (\top U b \lor c)))})$ | $(\top \lor (( p_\top \lor \bot) \land (\bot \land p_{\top U (b \lor c)}))) \land (\bot \land (\top \land p_\bot \land (\bot \lor p_{\neg (\top U (b\lor c))})))$ |


$$\begin{align}
\Delta(p_{\neg(a \land \neg (\top U (b\lor c)))}, a) =& \overline{\Delta(p_a, a) \land \Delta(p_{\neg (\top U (b\lor c)), a})}\\
 =&\overline{\Delta(p_a, a)} \lor \overline{\Delta(p_{\neg (\top U (b\lor c)), a})}\\
 =&\Delta(p_{\neg a}, a) \lor \Delta(p_{ (\top U (b\lor c)), a})\\
 =& p_\bot \lor (\bot \lor (\top \land p_{\top U (b \lor c)}))
\end{align}$$

$$\begin{align}
\Delta(p_{\top U (a \land \neg (\top U (b\lor c)))}, a) =& \Delta((a \land \neg (\top U (b\lor c))), a) \lor (\Delta(p_\top, a) \land \top U (a \land \neg (\top U (b\lor c))))\\
=& p_\top \land (\top \land (\bot \lor p_{\neg(\top U (b \lor c))})) \lor (\top \land p_{\top U (a \land \neg (\top U (b\lor c)))})
\end{align}$$

$$\begin{align}
\Delta(p_{\top U (a \land \neg (\top U (b\lor c)))}, b) =& \Delta((a \land \neg (\top U (b\lor c))), b) \lor (\Delta(p_\top, b) \land \top U (a \land \neg (\top U (b\lor c))))\\
=& (\bot \land ((p_\bot\land \top) \land(\bot \lor p_{\neg (\top U (b\lor c))}))) \lor (\top \land p_{\top U (a \land \neg (\top U (b\lor c)))})
\end{align}$$

---

$$\begin{align}
\Delta(p_{\neg(\top U (a \land \neg (\top U (b\lor c))))}, a) =& \overline{\Delta(p_{\top U (a \land \neg (\top U (b\lor c)))}, a)}\\
=& \overline{p_\top \land (\top \land (\bot \lor p_{\neg(\top U (b \lor c))})) \lor (\top \land p_{\top U (a \land \neg (\top U (b\lor c)))})}\\
=& \overline{p_\top} \lor (\overline{(\bot \lor (\bot \lor p_{\neg(\top U (b \lor c))}))} \land \overline{(\top \land p_{\top U (a \land \neg (\top U (b\lor c)))})}\\
=& p_\bot \lor (\top \land (\top \land p_{\top U (b \lor c)})) \land (\bot \lor p_{\neg (\top U (a \land \neg \top U (b \lor c)))})
\end{align}$$

---

